<?xml version="1.0"?>
<rdf:RDF xmlns="http://www.bioassayontology.org/bao/external/BAO_UO_import.owl#"
     xml:base="http://www.bioassayontology.org/bao/external/BAO_UO_import.owl"
     xmlns:obo="http://purl.obolibrary.org/obo/"
     xmlns:owl="http://www.w3.org/2002/07/owl#"
     xmlns:rdf="http://www.w3.org/1999/02/22-rdf-syntax-ns#"
     xmlns:xml="http://www.w3.org/XML/1998/namespace"
     xmlns:xsd="http://www.w3.org/2001/XMLSchema#"
     xmlns:rdfs="http://www.w3.org/2000/01/rdf-schema#"
     xmlns:oboInOwl="http://www.geneontology.org/formats/oboInOwl#">
    <owl:Ontology rdf:about="http://www.bioassayontology.org/bao/external/BAO_UO_import.owl"/>
    


    <!-- 
    ///////////////////////////////////////////////////////////////////////////////////////
    //
    // Annotation properties
    //
    ///////////////////////////////////////////////////////////////////////////////////////
     -->

    


    <!-- http://purl.obolibrary.org/obo/IAO_0000115 -->

    <owl:AnnotationProperty rdf:about="http://purl.obolibrary.org/obo/IAO_0000115">
        <rdfs:label>definition</rdfs:label>
    </owl:AnnotationProperty>
    


    <!-- http://purl.obolibrary.org/obo/IAO_0000412 -->

    <owl:AnnotationProperty rdf:about="http://purl.obolibrary.org/obo/IAO_0000412">
        <rdfs:label xml:lang="en">imported from</rdfs:label>
    </owl:AnnotationProperty>
    


    <!-- http://www.geneontology.org/formats/oboInOwl#created_by -->

    <owl:AnnotationProperty rdf:about="http://www.geneontology.org/formats/oboInOwl#created_by"/>
    


    <!-- http://www.geneontology.org/formats/oboInOwl#creation_date -->

    <owl:AnnotationProperty rdf:about="http://www.geneontology.org/formats/oboInOwl#creation_date"/>
    


    <!-- http://www.geneontology.org/formats/oboInOwl#hasAlternativeId -->

    <owl:AnnotationProperty rdf:about="http://www.geneontology.org/formats/oboInOwl#hasAlternativeId">
        <rdfs:label>has_alternative_id</rdfs:label>
    </owl:AnnotationProperty>
    


    <!-- http://www.geneontology.org/formats/oboInOwl#hasExactSynonym -->

    <owl:AnnotationProperty rdf:about="http://www.geneontology.org/formats/oboInOwl#hasExactSynonym">
        <rdfs:label>has_exact_synonym</rdfs:label>
    </owl:AnnotationProperty>
    


    <!-- http://www.geneontology.org/formats/oboInOwl#hasNarrowSynonym -->

    <owl:AnnotationProperty rdf:about="http://www.geneontology.org/formats/oboInOwl#hasNarrowSynonym">
        <rdfs:label>has_narrow_synonym</rdfs:label>
    </owl:AnnotationProperty>
    


    <!-- http://www.geneontology.org/formats/oboInOwl#hasOBONamespace -->

    <owl:AnnotationProperty rdf:about="http://www.geneontology.org/formats/oboInOwl#hasOBONamespace">
        <rdfs:label>has_obo_namespace</rdfs:label>
    </owl:AnnotationProperty>
    


    <!-- http://www.geneontology.org/formats/oboInOwl#id -->

    <owl:AnnotationProperty rdf:about="http://www.geneontology.org/formats/oboInOwl#id"/>
    


    <!-- http://www.geneontology.org/formats/oboInOwl#inSubset -->

    <owl:AnnotationProperty rdf:about="http://www.geneontology.org/formats/oboInOwl#inSubset">
        <rdfs:label>in_subset</rdfs:label>
    </owl:AnnotationProperty>
    


    <!-- http://www.w3.org/2000/01/rdf-schema#comment -->

    <owl:AnnotationProperty rdf:about="http://www.w3.org/2000/01/rdf-schema#comment"/>
    


    <!-- http://www.w3.org/2000/01/rdf-schema#label -->

    <owl:AnnotationProperty rdf:about="http://www.w3.org/2000/01/rdf-schema#label"/>
    


    <!-- 
    ///////////////////////////////////////////////////////////////////////////////////////
    //
    // Classes
    //
    ///////////////////////////////////////////////////////////////////////////////////////
     -->

    


    <!-- http://purl.obolibrary.org/obo/UO_0000001 -->

    <owl:Class rdf:about="http://purl.obolibrary.org/obo/UO_0000001">
        <obo:IAO_0000115>A unit which is a standard measure of the distance between two points.</obo:IAO_0000115>
        <obo:IAO_0000412 rdf:resource="http://purl.obolibrary.org/obo/uo.owl"/>
        <oboInOwl:created_by>george gkoutos</oboInOwl:created_by>
        <oboInOwl:hasOBONamespace>unit.ontology</oboInOwl:hasOBONamespace>
        <oboInOwl:id>UO:0000001</oboInOwl:id>
        <oboInOwl:inSubset rdf:resource="http://purl.oboInOwllibrary.org/oboInOwl/uo#unit_group_slim"/>
        <rdfs:label>length unit</rdfs:label>
    </owl:Class>
    


    <!-- http://purl.obolibrary.org/obo/UO_0000003 -->

    <owl:Class rdf:about="http://purl.obolibrary.org/obo/UO_0000003">
        <obo:IAO_0000115>A unit which is a standard measure of the dimension in which events occur in sequence.</obo:IAO_0000115>
        <obo:IAO_0000412 rdf:resource="http://purl.obolibrary.org/obo/uo.owl"/>
        <oboInOwl:created_by>george gkoutos</oboInOwl:created_by>
        <oboInOwl:hasAlternativeId>UO:0000149</oboInOwl:hasAlternativeId>
        <oboInOwl:hasExactSynonym>time derived unit</oboInOwl:hasExactSynonym>
        <oboInOwl:hasOBONamespace>unit.ontology</oboInOwl:hasOBONamespace>
        <oboInOwl:id>UO:0000003</oboInOwl:id>
        <oboInOwl:inSubset rdf:resource="http://purl.oboInOwllibrary.org/oboInOwl/uo#unit_group_slim"/>
        <rdfs:label>time unit</rdfs:label>
    </owl:Class>
    


    <!-- http://purl.obolibrary.org/obo/UO_0000005 -->

    <owl:Class rdf:about="http://purl.obolibrary.org/obo/UO_0000005">
        <obo:IAO_0000115>A unit which is a standard measure of the average kinetic energy of the particles in a sample of matter.</obo:IAO_0000115>
        <obo:IAO_0000412 rdf:resource="http://purl.obolibrary.org/obo/uo.owl"/>
        <oboInOwl:created_by>george gkoutos</oboInOwl:created_by>
        <oboInOwl:hasAlternativeId>UO:0000126</oboInOwl:hasAlternativeId>
        <oboInOwl:hasExactSynonym>temperature derived unit</oboInOwl:hasExactSynonym>
        <oboInOwl:hasOBONamespace>unit.ontology</oboInOwl:hasOBONamespace>
        <oboInOwl:id>UO:0000005</oboInOwl:id>
        <oboInOwl:inSubset rdf:resource="http://purl.oboInOwllibrary.org/oboInOwl/uo#unit_group_slim"/>
        <rdfs:label>temperature unit</rdfs:label>
    </owl:Class>
    


    <!-- http://purl.obolibrary.org/obo/UO_0000008 -->

    <owl:Class rdf:about="http://purl.obolibrary.org/obo/UO_0000008">
        <rdfs:subClassOf rdf:resource="http://purl.obolibrary.org/obo/UO_0000001"/>
        <obo:IAO_0000115>A length unit which is equal to the length of the path traveled by light in vacuum during a time interval of 1/299 792 458 of a second.</obo:IAO_0000115>
        <obo:IAO_0000412 rdf:resource="http://purl.obolibrary.org/obo/uo.owl"/>
        <oboInOwl:created_by>george gkoutos</oboInOwl:created_by>
        <oboInOwl:hasExactSynonym>m</oboInOwl:hasExactSynonym>
        <oboInOwl:hasExactSynonym>metre</oboInOwl:hasExactSynonym>
        <oboInOwl:hasOBONamespace>unit.ontology</oboInOwl:hasOBONamespace>
        <oboInOwl:id>UO:0000008</oboInOwl:id>
        <oboInOwl:inSubset rdf:resource="http://purl.oboInOwllibrary.org/oboInOwl/uo#unit_slim"/>
        <rdfs:label>meter</rdfs:label>
    </owl:Class>
    


    <!-- http://purl.obolibrary.org/obo/UO_0000010 -->

    <owl:Class rdf:about="http://purl.obolibrary.org/obo/UO_0000010">
        <rdfs:subClassOf rdf:resource="http://purl.obolibrary.org/obo/UO_0000003"/>
        <obo:IAO_0000115>A time unit which is equal to the duration of 9 192 631 770 periods of the radiation corresponding to the transition between the two hyperfine levels of the ground state of the caesium 133 atom.</obo:IAO_0000115>
        <obo:IAO_0000412 rdf:resource="http://purl.obolibrary.org/obo/uo.owl"/>
        <oboInOwl:created_by>george gkoutos</oboInOwl:created_by>
        <oboInOwl:hasExactSynonym>s</oboInOwl:hasExactSynonym>
        <oboInOwl:hasOBONamespace>unit.ontology</oboInOwl:hasOBONamespace>
        <oboInOwl:id>UO:0000010</oboInOwl:id>
        <oboInOwl:inSubset rdf:resource="http://purl.oboInOwllibrary.org/oboInOwl/uo#unit_slim"/>
        <rdfs:label>second</rdfs:label>
    </owl:Class>
    


    <!-- http://purl.obolibrary.org/obo/UO_0000012 -->

    <owl:Class rdf:about="http://purl.obolibrary.org/obo/UO_0000012">
        <rdfs:subClassOf rdf:resource="http://purl.obolibrary.org/obo/UO_0000005"/>
        <obo:IAO_0000115>A thermodynamic temperature unit which is equal to the fraction 1/273.16 of the thermodynamic temperature of the triple point of water.</obo:IAO_0000115>
        <obo:IAO_0000412 rdf:resource="http://purl.obolibrary.org/obo/uo.owl"/>
        <oboInOwl:created_by>george gkoutos</oboInOwl:created_by>
        <oboInOwl:hasExactSynonym>K</oboInOwl:hasExactSynonym>
        <oboInOwl:hasOBONamespace>unit.ontology</oboInOwl:hasOBONamespace>
        <oboInOwl:id>UO:0000012</oboInOwl:id>
        <oboInOwl:inSubset rdf:resource="http://purl.oboInOwllibrary.org/oboInOwl/uo#unit_slim"/>
        <rdfs:label>kelvin</rdfs:label>
    </owl:Class>
    


    <!-- http://purl.obolibrary.org/obo/UO_0000015 -->

    <owl:Class rdf:about="http://purl.obolibrary.org/obo/UO_0000015">
        <rdfs:subClassOf rdf:resource="http://purl.obolibrary.org/obo/UO_0000001"/>
        <obo:IAO_0000115>A length unit which is equal to one hundredth of a meter or 10^[-2] m.</obo:IAO_0000115>
        <obo:IAO_0000412 rdf:resource="http://purl.obolibrary.org/obo/uo.owl"/>
        <oboInOwl:created_by>george gkoutos</oboInOwl:created_by>
        <oboInOwl:hasExactSynonym>centimetre</oboInOwl:hasExactSynonym>
        <oboInOwl:hasExactSynonym>cm</oboInOwl:hasExactSynonym>
        <oboInOwl:hasOBONamespace>unit.ontology</oboInOwl:hasOBONamespace>
        <oboInOwl:id>UO:0000015</oboInOwl:id>
        <oboInOwl:inSubset rdf:resource="http://purl.oboInOwllibrary.org/oboInOwl/uo#unit_slim"/>
        <rdfs:label>centimeter</rdfs:label>
    </owl:Class>
    


    <!-- http://purl.obolibrary.org/obo/UO_0000016 -->

    <owl:Class rdf:about="http://purl.obolibrary.org/obo/UO_0000016">
        <rdfs:subClassOf rdf:resource="http://purl.obolibrary.org/obo/UO_0000001"/>
        <obo:IAO_0000115>A length unit which is equal to one thousandth of a meter or 10^[-3] m.</obo:IAO_0000115>
        <obo:IAO_0000412 rdf:resource="http://purl.obolibrary.org/obo/uo.owl"/>
        <oboInOwl:created_by>george gkoutos</oboInOwl:created_by>
        <oboInOwl:hasExactSynonym>micrometre</oboInOwl:hasExactSynonym>
        <oboInOwl:hasExactSynonym>mm</oboInOwl:hasExactSynonym>
        <oboInOwl:hasOBONamespace>unit.ontology</oboInOwl:hasOBONamespace>
        <oboInOwl:id>UO:0000016</oboInOwl:id>
        <oboInOwl:inSubset rdf:resource="http://purl.oboInOwllibrary.org/oboInOwl/uo#unit_slim"/>
        <rdfs:label>millimeter</rdfs:label>
    </owl:Class>
    


    <!-- http://purl.obolibrary.org/obo/UO_0000017 -->

    <owl:Class rdf:about="http://purl.obolibrary.org/obo/UO_0000017">
        <rdfs:subClassOf rdf:resource="http://purl.obolibrary.org/obo/UO_0000001"/>
        <obo:IAO_0000115>A length unit which is equal to one millionth of a meter or 10^[-6] m.</obo:IAO_0000115>
        <obo:IAO_0000412 rdf:resource="http://purl.obolibrary.org/obo/uo.owl"/>
        <oboInOwl:created_by>george gkoutos</oboInOwl:created_by>
        <oboInOwl:hasExactSynonym>micrometre</oboInOwl:hasExactSynonym>
        <oboInOwl:hasExactSynonym>micron</oboInOwl:hasExactSynonym>
        <oboInOwl:hasExactSynonym>um</oboInOwl:hasExactSynonym>
        <oboInOwl:hasOBONamespace>unit.ontology</oboInOwl:hasOBONamespace>
        <oboInOwl:id>UO:0000017</oboInOwl:id>
        <oboInOwl:inSubset rdf:resource="http://purl.oboInOwllibrary.org/oboInOwl/uo#unit_slim"/>
        <rdfs:label>micrometer</rdfs:label>
    </owl:Class>
    


    <!-- http://purl.obolibrary.org/obo/UO_0000018 -->

    <owl:Class rdf:about="http://purl.obolibrary.org/obo/UO_0000018">
        <rdfs:subClassOf rdf:resource="http://purl.obolibrary.org/obo/UO_0000001"/>
        <obo:IAO_0000115>A length unit which is equal to one thousandth of one millionth of a meter or 10^[-9] m.</obo:IAO_0000115>
        <obo:IAO_0000412 rdf:resource="http://purl.obolibrary.org/obo/uo.owl"/>
        <oboInOwl:created_by>george gkoutos</oboInOwl:created_by>
        <oboInOwl:hasExactSynonym>nanometre</oboInOwl:hasExactSynonym>
        <oboInOwl:hasExactSynonym>nm</oboInOwl:hasExactSynonym>
        <oboInOwl:hasOBONamespace>unit.ontology</oboInOwl:hasOBONamespace>
        <oboInOwl:id>UO:0000018</oboInOwl:id>
        <oboInOwl:inSubset rdf:resource="http://purl.oboInOwllibrary.org/oboInOwl/uo#unit_slim"/>
        <rdfs:label>nanometer</rdfs:label>
    </owl:Class>
    


    <!-- http://purl.obolibrary.org/obo/UO_0000019 -->

    <owl:Class rdf:about="http://purl.obolibrary.org/obo/UO_0000019">
        <rdfs:subClassOf rdf:resource="http://purl.obolibrary.org/obo/UO_0000001"/>
        <obo:IAO_0000115>A length unit which is equal to 10 [-10] m.</obo:IAO_0000115>
        <obo:IAO_0000412 rdf:resource="http://purl.obolibrary.org/obo/uo.owl"/>
        <oboInOwl:created_by>george gkoutos</oboInOwl:created_by>
        <oboInOwl:hasExactSynonym>Å</oboInOwl:hasExactSynonym>
        <oboInOwl:hasOBONamespace>unit.ontology</oboInOwl:hasOBONamespace>
        <oboInOwl:id>UO:0000019</oboInOwl:id>
        <oboInOwl:inSubset rdf:resource="http://purl.oboInOwllibrary.org/oboInOwl/uo#unit_slim"/>
        <rdfs:label>angstrom</rdfs:label>
    </owl:Class>
    


    <!-- http://purl.obolibrary.org/obo/UO_0000020 -->

    <owl:Class rdf:about="http://purl.obolibrary.org/obo/UO_0000020">
        <rdfs:subClassOf rdf:resource="http://purl.obolibrary.org/obo/UO_0000001"/>
        <obo:IAO_0000115>A length unit which is equal to 10^[-12] m.</obo:IAO_0000115>
        <obo:IAO_0000412 rdf:resource="http://purl.obolibrary.org/obo/uo.owl"/>
        <oboInOwl:created_by>george gkoutos</oboInOwl:created_by>
        <oboInOwl:hasExactSynonym>picometre</oboInOwl:hasExactSynonym>
        <oboInOwl:hasExactSynonym>pm</oboInOwl:hasExactSynonym>
        <oboInOwl:hasOBONamespace>unit.ontology</oboInOwl:hasOBONamespace>
        <oboInOwl:id>UO:0000020</oboInOwl:id>
        <oboInOwl:inSubset rdf:resource="http://purl.oboInOwllibrary.org/oboInOwl/uo#unit_slim"/>
        <rdfs:label>picometer</rdfs:label>
    </owl:Class>
    


    <!-- http://purl.obolibrary.org/obo/UO_0000027 -->

    <owl:Class rdf:about="http://purl.obolibrary.org/obo/UO_0000027">
        <rdfs:subClassOf rdf:resource="http://purl.obolibrary.org/obo/UO_0000005"/>
        <obo:IAO_0000115>A temperature unit which is equal to one kelvin degree. However, they have their zeros at different points. The centigrade scale has its zero at 273.15 K.</obo:IAO_0000115>
        <obo:IAO_0000412 rdf:resource="http://purl.obolibrary.org/obo/uo.owl"/>
        <oboInOwl:created_by>george gkoutos</oboInOwl:created_by>
        <oboInOwl:hasExactSynonym>C</oboInOwl:hasExactSynonym>
        <oboInOwl:hasOBONamespace>unit.ontology</oboInOwl:hasOBONamespace>
        <oboInOwl:id>UO:0000027</oboInOwl:id>
        <oboInOwl:inSubset rdf:resource="http://purl.oboInOwllibrary.org/oboInOwl/uo#unit_slim"/>
        <rdfs:label>degree Celsius</rdfs:label>
    </owl:Class>
    


    <!-- http://purl.obolibrary.org/obo/UO_0000028 -->

    <owl:Class rdf:about="http://purl.obolibrary.org/obo/UO_0000028">
        <rdfs:subClassOf rdf:resource="http://purl.obolibrary.org/obo/UO_0000003"/>
        <obo:IAO_0000115>A time unit which is equal to one thousandth of a second or 10^[-3] s.</obo:IAO_0000115>
        <obo:IAO_0000412 rdf:resource="http://purl.obolibrary.org/obo/uo.owl"/>
        <oboInOwl:created_by>george gkoutos</oboInOwl:created_by>
        <oboInOwl:hasExactSynonym>ms</oboInOwl:hasExactSynonym>
        <oboInOwl:hasOBONamespace>unit.ontology</oboInOwl:hasOBONamespace>
        <oboInOwl:id>UO:0000028</oboInOwl:id>
        <oboInOwl:inSubset rdf:resource="http://purl.oboInOwllibrary.org/oboInOwl/uo#unit_slim"/>
        <rdfs:label>millisecond</rdfs:label>
    </owl:Class>
    


    <!-- http://purl.obolibrary.org/obo/UO_0000029 -->

    <owl:Class rdf:about="http://purl.obolibrary.org/obo/UO_0000029">
        <rdfs:subClassOf rdf:resource="http://purl.obolibrary.org/obo/UO_0000003"/>
        <obo:IAO_0000115>A time unit which is equal to one millionth of a second or 10^[-6] s.</obo:IAO_0000115>
        <obo:IAO_0000412 rdf:resource="http://purl.obolibrary.org/obo/uo.owl"/>
        <oboInOwl:created_by>george gkoutos</oboInOwl:created_by>
        <oboInOwl:hasExactSynonym>us</oboInOwl:hasExactSynonym>
        <oboInOwl:hasOBONamespace>unit.ontology</oboInOwl:hasOBONamespace>
        <oboInOwl:id>UO:0000029</oboInOwl:id>
        <oboInOwl:inSubset rdf:resource="http://purl.oboInOwllibrary.org/oboInOwl/uo#unit_slim"/>
        <rdfs:label>microsecond</rdfs:label>
    </owl:Class>
    


    <!-- http://purl.obolibrary.org/obo/UO_0000030 -->

    <owl:Class rdf:about="http://purl.obolibrary.org/obo/UO_0000030">
        <rdfs:subClassOf rdf:resource="http://purl.obolibrary.org/obo/UO_0000003"/>
        <obo:IAO_0000115>A time unit which is equal to 10^[-12] s.</obo:IAO_0000115>
        <obo:IAO_0000412 rdf:resource="http://purl.obolibrary.org/obo/uo.owl"/>
        <oboInOwl:created_by>george gkoutos</oboInOwl:created_by>
        <oboInOwl:hasExactSynonym>ps</oboInOwl:hasExactSynonym>
        <oboInOwl:hasOBONamespace>unit.ontology</oboInOwl:hasOBONamespace>
        <oboInOwl:id>UO:0000030</oboInOwl:id>
        <oboInOwl:inSubset rdf:resource="http://purl.oboInOwllibrary.org/oboInOwl/uo#unit_slim"/>
        <rdfs:label>picosecond</rdfs:label>
    </owl:Class>
    


    <!-- http://purl.obolibrary.org/obo/UO_0000031 -->

    <owl:Class rdf:about="http://purl.obolibrary.org/obo/UO_0000031">
        <rdfs:subClassOf rdf:resource="http://purl.obolibrary.org/obo/UO_0000003"/>
        <obo:IAO_0000115>A time unit which is equal to 60 seconds.</obo:IAO_0000115>
        <obo:IAO_0000412 rdf:resource="http://purl.obolibrary.org/obo/uo.owl"/>
        <oboInOwl:created_by>george gkoutos</oboInOwl:created_by>
        <oboInOwl:hasExactSynonym>min</oboInOwl:hasExactSynonym>
        <oboInOwl:hasOBONamespace>unit.ontology</oboInOwl:hasOBONamespace>
        <oboInOwl:id>UO:0000031</oboInOwl:id>
        <oboInOwl:inSubset rdf:resource="http://purl.oboInOwllibrary.org/oboInOwl/uo#unit_slim"/>
        <rdfs:label>minute</rdfs:label>
    </owl:Class>
    


    <!-- http://purl.obolibrary.org/obo/UO_0000032 -->

    <owl:Class rdf:about="http://purl.obolibrary.org/obo/UO_0000032">
        <rdfs:subClassOf rdf:resource="http://purl.obolibrary.org/obo/UO_0000003"/>
        <obo:IAO_0000115>A time unit which is equal to 3600 seconds or 60 minutes.</obo:IAO_0000115>
        <obo:IAO_0000412 rdf:resource="http://purl.obolibrary.org/obo/uo.owl"/>
        <oboInOwl:created_by>george gkoutos</oboInOwl:created_by>
        <oboInOwl:hasExactSynonym>h</oboInOwl:hasExactSynonym>
        <oboInOwl:hasOBONamespace>unit.ontology</oboInOwl:hasOBONamespace>
        <oboInOwl:id>UO:0000032</oboInOwl:id>
        <oboInOwl:inSubset rdf:resource="http://purl.oboInOwllibrary.org/oboInOwl/uo#unit_slim"/>
        <rdfs:label>hour</rdfs:label>
    </owl:Class>
    


    <!-- http://purl.obolibrary.org/obo/UO_0000033 -->

    <owl:Class rdf:about="http://purl.obolibrary.org/obo/UO_0000033">
        <rdfs:subClassOf rdf:resource="http://purl.obolibrary.org/obo/UO_0000003"/>
        <obo:IAO_0000115>A time unit which is equal to 24 hours.</obo:IAO_0000115>
        <obo:IAO_0000412 rdf:resource="http://purl.obolibrary.org/obo/uo.owl"/>
        <oboInOwl:created_by>george gkoutos</oboInOwl:created_by>
        <oboInOwl:hasOBONamespace>unit.ontology</oboInOwl:hasOBONamespace>
        <oboInOwl:id>UO:0000033</oboInOwl:id>
        <oboInOwl:inSubset rdf:resource="http://purl.oboInOwllibrary.org/oboInOwl/uo#unit_slim"/>
        <rdfs:label>day</rdfs:label>
    </owl:Class>
    


    <!-- http://purl.obolibrary.org/obo/UO_0000034 -->

    <owl:Class rdf:about="http://purl.obolibrary.org/obo/UO_0000034">
        <rdfs:subClassOf rdf:resource="http://purl.obolibrary.org/obo/UO_0000003"/>
        <obo:IAO_0000115>A time unit which is equal to 7 days.</obo:IAO_0000115>
        <obo:IAO_0000412 rdf:resource="http://purl.obolibrary.org/obo/uo.owl"/>
        <oboInOwl:created_by>george gkoutos</oboInOwl:created_by>
        <oboInOwl:hasOBONamespace>unit.ontology</oboInOwl:hasOBONamespace>
        <oboInOwl:id>UO:0000034</oboInOwl:id>
        <oboInOwl:inSubset rdf:resource="http://purl.oboInOwllibrary.org/oboInOwl/uo#unit_slim"/>
        <rdfs:label>week</rdfs:label>
    </owl:Class>
    


    <!-- http://purl.obolibrary.org/obo/UO_0000035 -->

    <owl:Class rdf:about="http://purl.obolibrary.org/obo/UO_0000035">
        <rdfs:subClassOf rdf:resource="http://purl.obolibrary.org/obo/UO_0000003"/>
        <obo:IAO_0000115>A time unit which is approximately equal to the length of time of one of cycle of the moon&apos;s phases which in science is taken to be equal to 30 days.</obo:IAO_0000115>
        <obo:IAO_0000412 rdf:resource="http://purl.obolibrary.org/obo/uo.owl"/>
        <oboInOwl:created_by>george gkoutos</oboInOwl:created_by>
        <oboInOwl:hasOBONamespace>unit.ontology</oboInOwl:hasOBONamespace>
        <oboInOwl:id>UO:0000035</oboInOwl:id>
        <oboInOwl:inSubset rdf:resource="http://purl.oboInOwllibrary.org/oboInOwl/uo#unit_slim"/>
        <rdfs:label>month</rdfs:label>
    </owl:Class>
    


    <!-- http://purl.obolibrary.org/obo/UO_0000036 -->

    <owl:Class rdf:about="http://purl.obolibrary.org/obo/UO_0000036">
        <rdfs:subClassOf rdf:resource="http://purl.obolibrary.org/obo/UO_0000003"/>
        <obo:IAO_0000115>A time unit which is equal to 12 months which in science is taken to be equal to 365.25 days.</obo:IAO_0000115>
        <obo:IAO_0000412 rdf:resource="http://purl.obolibrary.org/obo/uo.owl"/>
        <oboInOwl:created_by>george gkoutos</oboInOwl:created_by>
        <oboInOwl:hasOBONamespace>unit.ontology</oboInOwl:hasOBONamespace>
        <oboInOwl:id>UO:0000036</oboInOwl:id>
        <oboInOwl:inSubset rdf:resource="http://purl.oboInOwllibrary.org/oboInOwl/uo#unit_slim"/>
        <rdfs:label>year</rdfs:label>
    </owl:Class>
    


    <!-- http://purl.obolibrary.org/obo/UO_0000051 -->

    <owl:Class rdf:about="http://purl.obolibrary.org/obo/UO_0000051">
        <obo:IAO_0000115>A unit which represents a standard measurement of how much of a given substance there is mixed with another substance.</obo:IAO_0000115>
        <obo:IAO_0000412 rdf:resource="http://purl.obolibrary.org/obo/uo.owl"/>
        <oboInOwl:created_by>george gkoutos</oboInOwl:created_by>
        <oboInOwl:hasOBONamespace>unit.ontology</oboInOwl:hasOBONamespace>
        <oboInOwl:id>UO:0000051</oboInOwl:id>
        <oboInOwl:inSubset rdf:resource="http://purl.oboInOwllibrary.org/oboInOwl/uo#unit_group_slim"/>
        <rdfs:label>concentration unit</rdfs:label>
    </owl:Class>
    


    <!-- http://purl.obolibrary.org/obo/UO_0000058 -->

    <owl:Class rdf:about="http://purl.obolibrary.org/obo/UO_0000058">
        <rdfs:subClassOf rdf:resource="http://purl.obolibrary.org/obo/UO_0000105"/>
        <obo:IAO_0000115>A unit which is a standard measure of the number of rotations in a given time.</obo:IAO_0000115>
        <obo:IAO_0000412 rdf:resource="http://purl.obolibrary.org/obo/uo.owl"/>
        <oboInOwl:created_by>george gkoutos</oboInOwl:created_by>
        <oboInOwl:hasOBONamespace>unit.ontology</oboInOwl:hasOBONamespace>
        <oboInOwl:id>UO:0000058</oboInOwl:id>
        <oboInOwl:inSubset rdf:resource="http://purl.oboInOwllibrary.org/oboInOwl/uo#unit_group_slim"/>
        <rdfs:label>rotational frequency unit</rdfs:label>
    </owl:Class>
    


    <!-- http://purl.obolibrary.org/obo/UO_0000061 -->

    <owl:Class rdf:about="http://purl.obolibrary.org/obo/UO_0000061">
        <rdfs:subClassOf rdf:resource="http://purl.obolibrary.org/obo/UO_0000051"/>
        <obo:IAO_0000115>A concentration unit which is a standard measure of the number of moles of a given substance per liter of solution.</obo:IAO_0000115>
        <obo:IAO_0000412 rdf:resource="http://purl.obolibrary.org/obo/uo.owl"/>
        <oboInOwl:created_by>george gkoutos</oboInOwl:created_by>
        <oboInOwl:hasOBONamespace>unit.ontology</oboInOwl:hasOBONamespace>
        <oboInOwl:id>UO:0000061</oboInOwl:id>
        <oboInOwl:inSubset rdf:resource="http://purl.oboInOwllibrary.org/oboInOwl/uo#unit_group_slim"/>
        <rdfs:label>unit of molarity</rdfs:label>
    </owl:Class>
    


    <!-- http://purl.obolibrary.org/obo/UO_0000062 -->

    <owl:Class rdf:about="http://purl.obolibrary.org/obo/UO_0000062">
        <rdfs:subClassOf rdf:resource="http://purl.obolibrary.org/obo/UO_0000061"/>
        <obo:IAO_0000115>A unit of concentration which expresses a concentration of 1 mole of solute per liter of solution (mol/L).</obo:IAO_0000115>
        <obo:IAO_0000412 rdf:resource="http://purl.obolibrary.org/obo/uo.owl"/>
        <oboInOwl:created_by>george gkoutos</oboInOwl:created_by>
        <oboInOwl:hasExactSynonym>M</oboInOwl:hasExactSynonym>
        <oboInOwl:hasOBONamespace>unit.ontology</oboInOwl:hasOBONamespace>
        <oboInOwl:id>UO:0000062</oboInOwl:id>
        <oboInOwl:inSubset rdf:resource="http://purl.oboInOwllibrary.org/oboInOwl/uo#unit_slim"/>
        <rdfs:label>molar</rdfs:label>
    </owl:Class>
    


    <!-- http://purl.obolibrary.org/obo/UO_0000063 -->

    <owl:Class rdf:about="http://purl.obolibrary.org/obo/UO_0000063">
        <rdfs:subClassOf rdf:resource="http://purl.obolibrary.org/obo/UO_0000061"/>
        <obo:IAO_0000115>A unit of molarity which is equal to one thousandth of a molar or 10^[-3] M.</obo:IAO_0000115>
        <obo:IAO_0000412 rdf:resource="http://purl.obolibrary.org/obo/uo.owl"/>
        <oboInOwl:created_by>george gkoutos</oboInOwl:created_by>
        <oboInOwl:hasExactSynonym>mM</oboInOwl:hasExactSynonym>
        <oboInOwl:hasOBONamespace>unit.ontology</oboInOwl:hasOBONamespace>
        <oboInOwl:id>UO:0000063</oboInOwl:id>
        <oboInOwl:inSubset rdf:resource="http://purl.oboInOwllibrary.org/oboInOwl/uo#unit_slim"/>
        <rdfs:label>millimolar</rdfs:label>
    </owl:Class>
    


    <!-- http://purl.obolibrary.org/obo/UO_0000064 -->

    <owl:Class rdf:about="http://purl.obolibrary.org/obo/UO_0000064">
        <rdfs:subClassOf rdf:resource="http://purl.obolibrary.org/obo/UO_0000061"/>
        <obo:IAO_0000115>A unit of molarity which is equal to one millionth of a molar or 10^[-6] M.</obo:IAO_0000115>
        <obo:IAO_0000412 rdf:resource="http://purl.obolibrary.org/obo/uo.owl"/>
        <oboInOwl:created_by>george gkoutos</oboInOwl:created_by>
        <oboInOwl:hasExactSynonym>uM</oboInOwl:hasExactSynonym>
        <oboInOwl:hasOBONamespace>unit.ontology</oboInOwl:hasOBONamespace>
        <oboInOwl:id>UO:0000064</oboInOwl:id>
        <oboInOwl:inSubset rdf:resource="http://purl.oboInOwllibrary.org/oboInOwl/uo#unit_slim"/>
        <rdfs:label>micromolar</rdfs:label>
    </owl:Class>
    


    <!-- http://purl.obolibrary.org/obo/UO_0000065 -->

    <owl:Class rdf:about="http://purl.obolibrary.org/obo/UO_0000065">
        <rdfs:subClassOf rdf:resource="http://purl.obolibrary.org/obo/UO_0000061"/>
        <obo:IAO_0000115>A unit of molarity which is equal to one thousandth of one millionth of a molar or 10^[-9] M.</obo:IAO_0000115>
        <obo:IAO_0000412 rdf:resource="http://purl.obolibrary.org/obo/uo.owl"/>
        <oboInOwl:created_by>george gkoutos</oboInOwl:created_by>
        <oboInOwl:hasExactSynonym>nM</oboInOwl:hasExactSynonym>
        <oboInOwl:hasOBONamespace>unit.ontology</oboInOwl:hasOBONamespace>
        <oboInOwl:id>UO:0000065</oboInOwl:id>
        <oboInOwl:inSubset rdf:resource="http://purl.oboInOwllibrary.org/oboInOwl/uo#unit_slim"/>
        <rdfs:label>nanomolar</rdfs:label>
    </owl:Class>
    


    <!-- http://purl.obolibrary.org/obo/UO_0000066 -->

    <owl:Class rdf:about="http://purl.obolibrary.org/obo/UO_0000066">
        <rdfs:subClassOf rdf:resource="http://purl.obolibrary.org/obo/UO_0000061"/>
        <obo:IAO_0000115>A unit of molarity which is equal to 10^[-12] M.</obo:IAO_0000115>
        <obo:IAO_0000412 rdf:resource="http://purl.obolibrary.org/obo/uo.owl"/>
        <oboInOwl:created_by>george gkoutos</oboInOwl:created_by>
        <oboInOwl:hasExactSynonym>pM</oboInOwl:hasExactSynonym>
        <oboInOwl:hasOBONamespace>unit.ontology</oboInOwl:hasOBONamespace>
        <oboInOwl:id>UO:0000066</oboInOwl:id>
        <oboInOwl:inSubset rdf:resource="http://purl.oboInOwllibrary.org/oboInOwl/uo#unit_slim"/>
        <rdfs:label>picomolar</rdfs:label>
    </owl:Class>
    


    <!-- http://purl.obolibrary.org/obo/UO_0000073 -->

    <owl:Class rdf:about="http://purl.obolibrary.org/obo/UO_0000073">
        <rdfs:subClassOf rdf:resource="http://purl.obolibrary.org/obo/UO_0000061"/>
        <obo:IAO_0000115>A unit of molarity which is equal to 10^[-15] M.</obo:IAO_0000115>
        <obo:IAO_0000412 rdf:resource="http://purl.obolibrary.org/obo/uo.owl"/>
        <oboInOwl:created_by>george gkoutos</oboInOwl:created_by>
        <oboInOwl:hasExactSynonym>fM</oboInOwl:hasExactSynonym>
        <oboInOwl:hasOBONamespace>unit.ontology</oboInOwl:hasOBONamespace>
        <oboInOwl:id>UO:0000073</oboInOwl:id>
        <oboInOwl:inSubset rdf:resource="http://purl.oboInOwllibrary.org/oboInOwl/uo#unit_slim"/>
        <rdfs:label>femtomolar</rdfs:label>
    </owl:Class>
    


    <!-- http://purl.obolibrary.org/obo/UO_0000092 -->

    <owl:Class rdf:about="http://purl.obolibrary.org/obo/UO_0000092">
        <rdfs:subClassOf rdf:resource="http://purl.obolibrary.org/obo/UO_0000058"/>
        <obo:IAO_0000115>A rotational frequency unit which is equal to the number complete turn in a period of time that equals to 1 second.</obo:IAO_0000115>
        <obo:IAO_0000412 rdf:resource="http://purl.obolibrary.org/obo/uo.owl"/>
        <oboInOwl:created_by>george gkoutos</oboInOwl:created_by>
        <oboInOwl:hasExactSynonym>1/s</oboInOwl:hasExactSynonym>
        <oboInOwl:hasNarrowSynonym>one turn per second</oboInOwl:hasNarrowSynonym>
        <oboInOwl:hasOBONamespace>unit.ontology</oboInOwl:hasOBONamespace>
        <oboInOwl:id>UO:0000092</oboInOwl:id>
        <oboInOwl:inSubset rdf:resource="http://purl.oboInOwllibrary.org/oboInOwl/uo#unit_slim"/>
        <rdfs:label>turns per second</rdfs:label>
    </owl:Class>
    


    <!-- http://purl.obolibrary.org/obo/UO_0000105 -->

    <owl:Class rdf:about="http://purl.obolibrary.org/obo/UO_0000105">
        <obo:IAO_0000115>A unit which is a standard measure of the number of repetitive actions in a particular time.</obo:IAO_0000115>
        <obo:IAO_0000412 rdf:resource="http://purl.obolibrary.org/obo/uo.owl"/>
        <oboInOwl:created_by>george gkoutos</oboInOwl:created_by>
        <oboInOwl:hasOBONamespace>unit.ontology</oboInOwl:hasOBONamespace>
        <oboInOwl:id>UO:0000105</oboInOwl:id>
        <oboInOwl:inSubset rdf:resource="http://purl.oboInOwllibrary.org/oboInOwl/uo#unit_group_slim"/>
        <rdfs:label>frequency unit</rdfs:label>
    </owl:Class>
    


    <!-- http://purl.obolibrary.org/obo/UO_0000106 -->

    <owl:Class rdf:about="http://purl.obolibrary.org/obo/UO_0000106">
        <rdfs:subClassOf rdf:resource="http://purl.obolibrary.org/obo/UO_0000105"/>
        <obo:IAO_0000115>A frequency unit which is equal to 1 complete cycle of a recurring phenomenon in 1 second.</obo:IAO_0000115>
        <obo:IAO_0000412 rdf:resource="http://purl.obolibrary.org/obo/uo.owl"/>
        <oboInOwl:created_by>george gkoutos</oboInOwl:created_by>
        <oboInOwl:hasExactSynonym>Hz</oboInOwl:hasExactSynonym>
        <oboInOwl:hasExactSynonym>s^1</oboInOwl:hasExactSynonym>
        <oboInOwl:hasOBONamespace>unit.ontology</oboInOwl:hasOBONamespace>
        <oboInOwl:id>UO:0000106</oboInOwl:id>
        <oboInOwl:inSubset rdf:resource="http://purl.oboInOwllibrary.org/oboInOwl/uo#unit_slim"/>
        <rdfs:label>hertz</rdfs:label>
    </owl:Class>
    


    <!-- http://purl.obolibrary.org/obo/UO_0000150 -->

    <owl:Class rdf:about="http://purl.obolibrary.org/obo/UO_0000150">
        <rdfs:subClassOf rdf:resource="http://purl.obolibrary.org/obo/UO_0000003"/>
        <obo:IAO_0000115>A time unit which is equal to one thousandth of one millionth of a second or 10^[-9] s.</obo:IAO_0000115>
        <obo:IAO_0000412 rdf:resource="http://purl.obolibrary.org/obo/uo.owl"/>
        <oboInOwl:created_by>george gkoutos</oboInOwl:created_by>
        <oboInOwl:hasExactSynonym>ns</oboInOwl:hasExactSynonym>
        <oboInOwl:hasOBONamespace>unit.ontology</oboInOwl:hasOBONamespace>
        <oboInOwl:id>UO:0000150</oboInOwl:id>
        <oboInOwl:inSubset rdf:resource="http://purl.oboInOwllibrary.org/oboInOwl/uo#unit_slim"/>
        <rdfs:label>nanosecond</rdfs:label>
    </owl:Class>
    


    <!-- http://purl.obolibrary.org/obo/UO_0000151 -->

    <owl:Class rdf:about="http://purl.obolibrary.org/obo/UO_0000151">
        <rdfs:subClassOf rdf:resource="http://purl.obolibrary.org/obo/UO_0000003"/>
        <obo:IAO_0000115>A time unit which is equal to 100 years.</obo:IAO_0000115>
        <obo:IAO_0000412 rdf:resource="http://purl.obolibrary.org/obo/uo.owl"/>
        <oboInOwl:created_by>george gkoutos</oboInOwl:created_by>
        <oboInOwl:hasOBONamespace>unit.ontology</oboInOwl:hasOBONamespace>
        <oboInOwl:id>UO:0000151</oboInOwl:id>
        <oboInOwl:inSubset rdf:resource="http://purl.oboInOwllibrary.org/oboInOwl/uo#unit_slim"/>
        <rdfs:label>century</rdfs:label>
    </owl:Class>
    


    <!-- http://purl.obolibrary.org/obo/UO_0000152 -->

    <owl:Class rdf:about="http://purl.obolibrary.org/obo/UO_0000152">
        <rdfs:subClassOf rdf:resource="http://purl.obolibrary.org/obo/UO_0000003"/>
        <obo:IAO_0000115>A time unit which represents the period over which the activity or concentration of a specified chemical or element falls to half its original activity or concentration.</obo:IAO_0000115>
        <obo:IAO_0000412 rdf:resource="http://purl.obolibrary.org/obo/uo.owl"/>
        <oboInOwl:created_by>george gkoutos</oboInOwl:created_by>
        <oboInOwl:hasOBONamespace>unit.ontology</oboInOwl:hasOBONamespace>
        <oboInOwl:id>UO:0000152</oboInOwl:id>
        <oboInOwl:inSubset rdf:resource="http://purl.oboInOwllibrary.org/oboInOwl/uo#unit_slim"/>
        <rdfs:comment>Typically applied to the half life of radioactive atoms but also applicable to any other situation where the population is of molecules of diminishing concentration or activity.</rdfs:comment>
        <rdfs:label>half life</rdfs:label>
    </owl:Class>
    


    <!-- http://purl.obolibrary.org/obo/UO_0000163 -->

    <owl:Class rdf:about="http://purl.obolibrary.org/obo/UO_0000163">
        <rdfs:subClassOf rdf:resource="http://purl.obolibrary.org/obo/UO_0000051"/>
        <obo:IAO_0000115>A dimensionless concentration unit which denotes the mass of a substance in a mixture as a percentage of the mass of the entire mixture.</obo:IAO_0000115>
        <obo:IAO_0000412 rdf:resource="http://purl.obolibrary.org/obo/uo.owl"/>
        <oboInOwl:created_by>george gkoutos</oboInOwl:created_by>
        <oboInOwl:hasExactSynonym>w/w</oboInOwl:hasExactSynonym>
        <oboInOwl:hasExactSynonym>weight-weight percentage</oboInOwl:hasExactSynonym>
        <oboInOwl:hasOBONamespace>unit.ontology</oboInOwl:hasOBONamespace>
        <oboInOwl:id>UO:0000163</oboInOwl:id>
        <oboInOwl:inSubset rdf:resource="http://purl.oboInOwllibrary.org/oboInOwl/uo#unit_slim"/>
        <rdfs:label>mass percentage</rdfs:label>
    </owl:Class>
    


    <!-- http://purl.obolibrary.org/obo/UO_0000180 -->

    <owl:Class rdf:about="http://purl.obolibrary.org/obo/UO_0000180">
        <rdfs:subClassOf rdf:resource="http://purl.obolibrary.org/obo/UO_0000051"/>
        <obo:IAO_0000115>A concentration unit which is a standard measure of the mass of a substance in a given volume (density).</obo:IAO_0000115>
        <obo:IAO_0000412 rdf:resource="http://purl.obolibrary.org/obo/uo.owl"/>
        <oboInOwl:created_by>george gkoutos</oboInOwl:created_by>
        <oboInOwl:hasOBONamespace>unit.ontology</oboInOwl:hasOBONamespace>
        <oboInOwl:id>UO:0000180</oboInOwl:id>
        <oboInOwl:inSubset rdf:resource="http://purl.oboInOwllibrary.org/oboInOwl/uo#unit_slim"/>
        <rdfs:comment>For units and further information look under the mass density unit. For a sample of a specific pure elemental substance, the concentration is directly proportional to the density. However, concentration is not proportional to density in general.</rdfs:comment>
        <rdfs:label>mass per unit volume</rdfs:label>
    </owl:Class>
    


    <!-- http://purl.obolibrary.org/obo/UO_0000186 -->

    <owl:Class rdf:about="http://purl.obolibrary.org/obo/UO_0000186">
        <obo:IAO_0000115>A unit which is a standard measure of physical quantity consisting of only a numerical number without any units.</obo:IAO_0000115>
        <obo:IAO_0000412 rdf:resource="http://purl.obolibrary.org/obo/uo.owl"/>
        <oboInOwl:created_by>george gkoutos</oboInOwl:created_by>
        <oboInOwl:hasOBONamespace>unit.ontology</oboInOwl:hasOBONamespace>
        <oboInOwl:id>UO:0000186</oboInOwl:id>
        <oboInOwl:inSubset rdf:resource="http://purl.oboInOwllibrary.org/oboInOwl/uo#unit_group_slim"/>
        <rdfs:label>dimensionless unit</rdfs:label>
    </owl:Class>
    


    <!-- http://purl.obolibrary.org/obo/UO_0000187 -->

    <owl:Class rdf:about="http://purl.obolibrary.org/obo/UO_0000187">
        <rdfs:subClassOf rdf:resource="http://purl.obolibrary.org/obo/UO_0000190"/>
        <obo:IAO_0000115>A dimensionless ratio unit which denotes numbers as fractions of 100.</obo:IAO_0000115>
        <obo:IAO_0000412 rdf:resource="http://purl.obolibrary.org/obo/uo.owl"/>
        <oboInOwl:created_by>george gkoutos</oboInOwl:created_by>
        <oboInOwl:hasExactSynonym>%</oboInOwl:hasExactSynonym>
        <oboInOwl:hasOBONamespace>unit.ontology</oboInOwl:hasOBONamespace>
        <oboInOwl:id>UO:0000187</oboInOwl:id>
        <oboInOwl:inSubset rdf:resource="http://purl.oboInOwllibrary.org/oboInOwl/uo#unit_group_slim"/>
        <rdfs:label>percent</rdfs:label>
    </owl:Class>
    


    <!-- http://purl.obolibrary.org/obo/UO_0000190 -->

    <owl:Class rdf:about="http://purl.obolibrary.org/obo/UO_0000190">
        <rdfs:subClassOf rdf:resource="http://purl.obolibrary.org/obo/UO_0000186"/>
        <obo:IAO_0000115>A dimensionless unit which denotes an amount or magnitude of one quantity relative to another.</obo:IAO_0000115>
        <obo:IAO_0000412 rdf:resource="http://purl.obolibrary.org/obo/uo.owl"/>
        <oboInOwl:created_by>george gkoutos</oboInOwl:created_by>
        <oboInOwl:hasOBONamespace>unit.ontology</oboInOwl:hasOBONamespace>
        <oboInOwl:id>UO:0000190</oboInOwl:id>
        <oboInOwl:inSubset rdf:resource="http://purl.oboInOwllibrary.org/oboInOwl/uo#unit_group_slim"/>
        <rdfs:label>ratio</rdfs:label>
    </owl:Class>
    


    <!-- http://purl.obolibrary.org/obo/UO_0000195 -->

    <owl:Class rdf:about="http://purl.obolibrary.org/obo/UO_0000195">
        <rdfs:subClassOf rdf:resource="http://purl.obolibrary.org/obo/UO_0000005"/>
        <obo:IAO_0000115>A temperature unit which is equal to 5/9ths of a kelvin. Negative 40 degrees Fahrenheit is equal to negative 40 degrees Celsius.</obo:IAO_0000115>
        <obo:IAO_0000412 rdf:resource="http://purl.obolibrary.org/obo/uo.owl"/>
        <oboInOwl:created_by>george gkoutos</oboInOwl:created_by>
        <oboInOwl:hasExactSynonym>F</oboInOwl:hasExactSynonym>
        <oboInOwl:hasOBONamespace>unit.ontology</oboInOwl:hasOBONamespace>
        <oboInOwl:id>UO:0000195</oboInOwl:id>
        <oboInOwl:inSubset rdf:resource="http://purl.oboInOwllibrary.org/oboInOwl/uo#unit_slim"/>
        <rdfs:comment>In this scale, the freezing point of water is 32 degrees Fahrenheit and the boiling point is 212 degrees, placing the boiling and freezing points of water 180 degrees apart. -40 degrees Fahrenheit is equal to -40 degrees Celsius.</rdfs:comment>
        <rdfs:label>degree Fahrenheit</rdfs:label>
    </owl:Class>
    


    <!-- http://purl.obolibrary.org/obo/UO_0000196 -->

    <owl:Class rdf:about="http://purl.obolibrary.org/obo/UO_0000196">
        <rdfs:subClassOf rdf:resource="http://purl.obolibrary.org/obo/UO_0000051"/>
        <obo:IAO_0000115>A dimensionless concentration notation which denotes the acidity of a solution in terms of activity of hydrogen ions (H+).</obo:IAO_0000115>
        <obo:IAO_0000412 rdf:resource="http://purl.obolibrary.org/obo/uo.owl"/>
        <oboInOwl:created_by>george gkoutos</oboInOwl:created_by>
        <oboInOwl:hasOBONamespace>unit.ontology</oboInOwl:hasOBONamespace>
        <oboInOwl:id>UO:0000196</oboInOwl:id>
        <oboInOwl:inSubset rdf:resource="http://purl.oboInOwllibrary.org/oboInOwl/uo#unit_slim"/>
        <rdfs:label>pH</rdfs:label>
    </owl:Class>
    


    <!-- http://purl.obolibrary.org/obo/UO_0000200 -->

    <owl:Class rdf:about="http://purl.obolibrary.org/obo/UO_0000200">
        <rdfs:subClassOf rdf:resource="http://purl.obolibrary.org/obo/UO_0000051"/>
        <obo:IAO_0000115>A concentration unit which denotes the average cell number in a given volume.</obo:IAO_0000115>
        <obo:IAO_0000412 rdf:resource="http://purl.obolibrary.org/obo/uo.owl"/>
        <oboInOwl:created_by>george gkoutos</oboInOwl:created_by>
        <oboInOwl:hasOBONamespace>unit.ontology</oboInOwl:hasOBONamespace>
        <oboInOwl:id>UO:0000200</oboInOwl:id>
        <oboInOwl:inSubset rdf:resource="http://purl.oboInOwllibrary.org/oboInOwl/uo#unit_group_slim"/>
        <rdfs:label>cell concentration unit</rdfs:label>
    </owl:Class>
    


    <!-- http://purl.obolibrary.org/obo/UO_0000201 -->

    <owl:Class rdf:about="http://purl.obolibrary.org/obo/UO_0000201">
        <rdfs:subClassOf rdf:resource="http://purl.obolibrary.org/obo/UO_0000200"/>
        <obo:IAO_0000115>A unit of cell concentration which is equal to one cell in a volume of 1 milliliter.</obo:IAO_0000115>
        <obo:IAO_0000412 rdf:resource="http://purl.obolibrary.org/obo/uo.owl"/>
        <oboInOwl:created_by>george gkoutos</oboInOwl:created_by>
        <oboInOwl:hasExactSynonym>cells per millilitre</oboInOwl:hasExactSynonym>
        <oboInOwl:hasExactSynonym>cells per ml</oboInOwl:hasExactSynonym>
        <oboInOwl:hasOBONamespace>unit.ontology</oboInOwl:hasOBONamespace>
        <oboInOwl:id>UO:0000201</oboInOwl:id>
        <oboInOwl:inSubset rdf:resource="http://purl.oboInOwllibrary.org/oboInOwl/uo#unit_slim"/>
        <rdfs:label>cells per milliliter</rdfs:label>
    </owl:Class>
    


    <!-- http://purl.obolibrary.org/obo/UO_0000202 -->

    <owl:Class rdf:about="http://purl.obolibrary.org/obo/UO_0000202">
        <rdfs:subClassOf rdf:resource="http://purl.obolibrary.org/obo/UO_0000051"/>
        <obo:IAO_0000115>A concentration unit which is a standard measure of the amount of the action of a catalyst in a given volume.</obo:IAO_0000115>
        <obo:IAO_0000412 rdf:resource="http://purl.obolibrary.org/obo/uo.owl"/>
        <oboInOwl:created_by>george gkoutos</oboInOwl:created_by>
        <oboInOwl:hasOBONamespace>unit.ontology</oboInOwl:hasOBONamespace>
        <oboInOwl:id>UO:0000202</oboInOwl:id>
        <oboInOwl:inSubset rdf:resource="http://purl.oboInOwllibrary.org/oboInOwl/uo#unit_group_slim"/>
        <rdfs:label>catalytic (activity) concentration unit</rdfs:label>
    </owl:Class>
    


    <!-- http://purl.obolibrary.org/obo/UO_0000203 -->

    <owl:Class rdf:about="http://purl.obolibrary.org/obo/UO_0000203">
        <rdfs:subClassOf rdf:resource="http://purl.obolibrary.org/obo/UO_0000202"/>
        <obo:IAO_0000115>A catalytic (activity) concentration unit which is equal to 1 katal activity of a catalyst in a given volume of one cubic meter.</obo:IAO_0000115>
        <obo:IAO_0000412 rdf:resource="http://purl.obolibrary.org/obo/uo.owl"/>
        <oboInOwl:created_by>george gkoutos</oboInOwl:created_by>
        <oboInOwl:hasExactSynonym>kat/m^[3]</oboInOwl:hasExactSynonym>
        <oboInOwl:hasExactSynonym>katal per cubic metre</oboInOwl:hasExactSynonym>
        <oboInOwl:hasOBONamespace>unit.ontology</oboInOwl:hasOBONamespace>
        <oboInOwl:id>UO:0000203</oboInOwl:id>
        <oboInOwl:inSubset rdf:resource="http://purl.oboInOwllibrary.org/oboInOwl/uo#unit_slim"/>
        <rdfs:label>katal per cubic meter</rdfs:label>
    </owl:Class>
    


    <!-- http://purl.obolibrary.org/obo/UO_0000204 -->

    <owl:Class rdf:about="http://purl.obolibrary.org/obo/UO_0000204">
        <rdfs:subClassOf rdf:resource="http://purl.obolibrary.org/obo/UO_0000202"/>
        <obo:IAO_0000115>A catalytic (activity) concentration unit which is equal to 1 katal activity of a catalyst in a given volume of one thousandth of a cubic meter.</obo:IAO_0000115>
        <obo:IAO_0000412 rdf:resource="http://purl.obolibrary.org/obo/uo.owl"/>
        <oboInOwl:created_by>george gkoutos</oboInOwl:created_by>
        <oboInOwl:hasExactSynonym>kat/l</oboInOwl:hasExactSynonym>
        <oboInOwl:hasExactSynonym>katal per litre</oboInOwl:hasExactSynonym>
        <oboInOwl:hasOBONamespace>unit.ontology</oboInOwl:hasOBONamespace>
        <oboInOwl:id>UO:0000204</oboInOwl:id>
        <oboInOwl:inSubset rdf:resource="http://purl.oboInOwllibrary.org/oboInOwl/uo#unit_slim"/>
        <rdfs:label>katal per liter</rdfs:label>
    </owl:Class>
    


    <!-- http://purl.obolibrary.org/obo/UO_0000316 -->

    <owl:Class rdf:about="http://purl.obolibrary.org/obo/UO_0000316">
        <rdfs:subClassOf rdf:resource="http://purl.obolibrary.org/obo/UO_0000200"/>
        <obo:IAO_0000115>A unit of cell concentration which is equal to one cell in a volume of 1 microliter.</obo:IAO_0000115>
        <obo:IAO_0000412 rdf:resource="http://purl.obolibrary.org/obo/uo.owl"/>
        <oboInOwl:created_by>gkoutos</oboInOwl:created_by>
        <oboInOwl:creation_date>2013-03-12T12:34:17Z</oboInOwl:creation_date>
        <oboInOwl:hasExactSynonym>cells per microlitre</oboInOwl:hasExactSynonym>
        <oboInOwl:hasExactSynonym>cells per ul</oboInOwl:hasExactSynonym>
        <oboInOwl:hasOBONamespace>unit.ontology</oboInOwl:hasOBONamespace>
        <oboInOwl:id>UO:0000316</oboInOwl:id>
        <rdfs:label>cells per microliter</rdfs:label>
    </owl:Class>
    


    <!-- http://purl.obolibrary.org/obo/UO_0000317 -->

    <owl:Class rdf:about="http://purl.obolibrary.org/obo/UO_0000317">
        <rdfs:subClassOf rdf:resource="http://purl.obolibrary.org/obo/UO_0000200"/>
        <obo:IAO_0000115>A unit of cell concentration which is equal to 1 cell in a well or discrete container of arbitrary volume.</obo:IAO_0000115>
        <obo:IAO_0000412 rdf:resource="http://purl.obolibrary.org/obo/uo.owl"/>
        <oboInOwl:created_by>gkoutos</oboInOwl:created_by>
        <oboInOwl:creation_date>2013-03-12T12:46:20Z</oboInOwl:creation_date>
        <oboInOwl:hasOBONamespace>unit.ontology</oboInOwl:hasOBONamespace>
        <oboInOwl:id>UO:0000317</oboInOwl:id>
        <rdfs:label>cells per well</rdfs:label>
    </owl:Class>
</rdf:RDF>



<!-- Generated by the OWL API (version 4.5.29.2024-05-13T12:11:03Z) https://github.com/owlcs/owlapi -->

